<?xml version="1.0" encoding="UTF-8"?>
<!-- 
    WARNING:  THIS IS A WORKING DRAFT ONTOLOGY AND STILL UNDER DEVELOPMENT, this file will change frequently and significantly as development continues.
    
    Note:  http://artframe.biblioteko-o.org/ is a placeholder (fake) namespace for the LD4P/L ArtFrame Materials ontology extension until a proper home is found
  -->

<rdf:RDF xmlns="http://artframe.biblioteko-o.org/" xmlns:bf="http://id.loc.gov/ontologies/bibframe/"
    xmlns:bib="http://bibliotek-o.org/ontology/" xmlns:dcterms="http://purl.org/dc/terms/"
    xmlns:owl="http://www.w3.org/2002/07/owl#"
    xmlns:rdf="http://www.w3.org/1999/02/22-rdf-syntax-ns#"
    xmlns:rdfs="http://www.w3.org/2000/01/rdf-schema#"
    xmlns:skos="http://www.w3.org/2004/02/skos/core#" xmlns:xsd="http://www.w3.org/2001/XMLSchema#"
    xmlns:foaf="http://xmlns.com/foaf/0.1#" xmlns:vann="http://purl.org/vocab/vann/"
    xmlns:voaf="http://purl.org/vocommons/voaf#">

    <!-- ONTOLOGY DECLARATION -->

    <owl:Ontology rdf:about="http://artframe.biblioteko-o.org/">
        <owl:versionInfo rdf:datatype="http://www.w3.org/2001/XMLSchema#string">Version
            0.0</owl:versionInfo>
        <rdfs:label xml:lang="en">ArtFrame: extension ontology for describing art
            materials</rdfs:label>
        <vann:preferredNamespacePrefix>af</vann:preferredNamespacePrefix>
        <rdfs:comment xml:lang="en">ArtFrame is an extension ontology of the bibliotek-o BIBFRAME
            2.0 extension ontology for use in describing two-dimenstional and three-dimensional art
            objects</rdfs:comment>
        <voaf:extends rdf:resource="http://bibliotek-o.org/ontology/"/>
        <voaf:specializes rdf:resource="http://bibliotek-o.org/ontology/"/>
    </owl:Ontology>


    <!-- CLASSES -->

    <owl:Class rdf:about="http://artframe.biblioteko-o.org/MeasurementGroup">
        <rdfs:label>Measurement Group</rdfs:label>
        <skos:definition xml:lang="en-us">A set of measurements pertaining to a specific resource,
            part of a resource, or resource in a particular arrangement. For example, a book may
            have a specified height, width, length, and/or weight, which are all attached to a
            MeasurementGroup; the binding may have measurements specified independently, which would
            constitute another MeasurementGroup. A MeasurementGroup has one or more specific
            Measurements attached to it.</skos:definition>
    </owl:Class>

    <owl:Class rdf:about="http://artframe.biblioteko-o.org/Measurement">
        <rdfs:label>Measurement</rdfs:label>
        <skos:definition xml:lang="en-us">The measurement of a single aspect of a resource,
            including value, units, and the aspect measured. For example, a book may have a height
            (aspect) of 10 (value) centimeters (units). Each such measurement is attached to a
            MeasurementGroup.</skos:definition>
    </owl:Class>

    <owl:Class rdf:about="http://artframe.biblioteko-o.org/Arrangement">
        <rdfs:label>Arrangement</rdfs:label>
        <skos:definition xml:lang="en-us">The arrangement, organization, or configuration of a
            single object or collection of objects. For example, a parchment may be rolled or
            unrolled; a collection of visual materials has a specific arrangement; computer files
            are organized and ordered in a specific way.</skos:definition>
    </owl:Class>

    <owl:Class rdf:about="http://artframe.biblioteko-o.org/ConditionAssessmentActivity">
        <rdfs:label>Condition Assessment Activity</rdfs:label>
        <skos:definition xml:lang="en-us">The activity of assessing and documenting the physical
            condition of an item, including damage, material vulnerabilities, special storage
            requirements, etc. This activity outputs a ConditionAssessment.</skos:definition>
        <rdfs:subClassOf rdf:resource="http://bibliotek-o.org/1.1/ontology/Activity"/>
    </owl:Class>

    <owl:Class rdf:about="http://artframe.biblioteko-o.org/ConditionAssessment">
        <rdfs:label>Condition Assessment</rdfs:label>
        <skos:definition xml:lang="en-us">Assessment and/or documentation of the physical condition
            of an item, including damage, material vulnerabilities, special storage requirements,
            etc. The assessment is generally the output of a condition assessment activity, and may
            or may not result in a conservator activity.</skos:definition>
    </owl:Class>

    <owl:Class rdf:about="http://artframe.biblioteko-o.org/PhysicalCondition">
        <rdfs:label>Physical Conditiont</rdfs:label>
        <skos:definition xml:lang="en-us">One specific aspect of the condition of an object or part
            of an object, including perceptible or measurable characteristics such as physical
            appearance, level of damage, quality, or completeness.</skos:definition>
    </owl:Class>

    <!-- OBJECT PROPERTIES -->

    <owl:ObjectProperty rdf:about="http://artframe.biblioteko-o.org/hasMeasurementGroup">
        <rdfs:label xml:lang="en">has measurement group</rdfs:label>
        <skos:definition xml:lang="en">The relationship of a resource to a measurement group,
            indicating that the measurement group applies to the resource.</skos:definition>
        <rdfs:range rdf:resource="http://artframe.biblioteko-o.org/MeasurementGroup"/>
        <owl:inverseOf rdf:resource="http://artframe.biblioteko-o.org/isMeasurementGroupOf"/>
    </owl:ObjectProperty>

    <owl:ObjectProperty rdf:about="http://artframe.biblioteko-o.org/isMeasurementGroupOf">
        <rdfs:label xml:lang="en">is measurement group of</rdfs:label>
        <skos:definition xml:lang="en">The relationship of a measurement group to a resource,
            indicating that the measurement group applies to the resource.</skos:definition>
        <rdfs:domain rdf:resource="http://artframe.biblioteko-o.org/MeasurementGroup"/>
        <owl:inverseOf rdf:resource="http://artframe.biblioteko-o.org/hasMeasurementGroup"/>
    </owl:ObjectProperty>

    <owl:ObjectProperty rdf:about="http://artframe.biblioteko-o.org/hasMeasurement">
        <rdfs:label xml:lang="en">has measurement</rdfs:label>
        <skos:definition xml:lang="en">The relationship of a MeasurementGroup to a Measurement,
            indicating that the Measurement is one part of the MeasurementGroup.</skos:definition>
        <rdfs:range rdf:resource="http://artframe.biblioteko-o.org/Measurement"/>
        <owl:inverseOf rdf:resource="http://artframe.biblioteko-o.org/isMeasurementOf"/>
    </owl:ObjectProperty>

    <owl:ObjectProperty rdf:about="http://artframe.biblioteko-o.org/isMeasurementOf">
        <rdfs:label xml:lang="en">is measurement of</rdfs:label>
        <skos:definition xml:lang="en">The relationship of a Measurement to a MeasurementGroup,
            indicating that the Measurement is one part of the MeasurementGroup.</skos:definition>
        <rdfs:domain rdf:resource="http://artframe.biblioteko-o.org/Measurement"/>
        <rdfs:range rdf:resource="http://artframe.biblioteko-o.org/MeasurementGroup"/>
        <owl:inverseOf rdf:resource="http://artframe.biblioteko-o.org/hasMeasurement"/>
    </owl:ObjectProperty>

    <owl:ObjectProperty rdf:about="http://artframe.biblioteko-o.org/measures">
        <rdfs:label xml:lang="en">measures</rdfs:label>
        <skos:definition xml:lang="en">The relationship between a Measurement and the dimension or
            other aspect of a resource that is measured by this Measurement. For example, a
            Measurement may specify the length, height, weight, file size, etc. of a
            resource.</skos:definition>
        <rdfs:domain rdf:resource="http://artframe.biblioteko-o.org/Measurement"/>
        <owl:inverseOf rdf:resource="http://artframe.biblioteko-o.org/measuredBy"/>
    </owl:ObjectProperty>

    <owl:ObjectProperty rdf:about="http://artframe.biblioteko-o.org/measuredBy">
        <rdfs:label xml:lang="en">measured by</rdfs:label>
        <skos:definition xml:lang="en">The relationship between a dimension or other aspect of a
            resource and the Measurement that measures it. For example, the length, height, weight,
            file size, etc. of a resource may be the aspect that is measured by a particular
            Measurement.</skos:definition>
        <rdfs:range rdf:resource="http://artframe.biblioteko-o.org/Measurement"/>
        <owl:inverseOf rdf:resource="http://artframe.biblioteko-o.org/measures"/>
    </owl:ObjectProperty>

    <owl:ObjectProperty rdf:about="http://artframe.biblioteko-o.org/hasUnit">
        <rdfs:label xml:lang="en">has unit</rdfs:label>
        <skos:definition xml:lang="en">Relationship between the measurement and the unit used to
            express the measurement.</skos:definition>
        <owl:inverseOf rdf:resource="http://artframe.biblioteko-o.org/isUnitOf"/>
    </owl:ObjectProperty>

    <owl:ObjectProperty rdf:about="http://artframe.biblioteko-o.org/isUnitOf">
        <rdfs:label xml:lang="en">is unit of</rdfs:label>
        <skos:definition xml:lang="en">Relationship between the measurement and the unit used to
            express the measurement.</skos:definition>
        <owl:inverseOf rdf:resource="http://artframe.biblioteko-o.org/hasUnit"/>
    </owl:ObjectProperty>

    <owl:ObjectProperty rdf:about="http://artframe.biblioteko-o.org/hasArrangement">
        <rdfs:label xml:lang="en">has arrangement</rdfs:label>
        <skos:definition xml:lang="en">Relationship between the resource and a specified
            arrangement, organization, or configuration of it.</skos:definition>
        <rdfs:range rdf:resource="http://artframe.biblioteko-o.org/Arranegement"/>
        <owl:inverseOf rdf:resource="http://artframe.biblioteko-o.org/isArrangementOf"/>
    </owl:ObjectProperty>

    <owl:ObjectProperty rdf:about="http://artframe.biblioteko-o.org/isArrangementOf">
        <rdfs:label xml:lang="en">is arrangement of</rdfs:label>
        <skos:definition xml:lang="en">Relationship between a specified arrangement, organization,
            or configuration and a resource.</skos:definition>
        <rdfs:domain rdf:resource="http://artframe.biblioteko-o.org/Arranegement"/>
        <owl:inverseOf rdf:resource="http://artframe.biblioteko-o.org/hasArrangement"/>
    </owl:ObjectProperty>

    <owl:ObjectProperty rdf:about="http://artframe.biblioteko-o.org/cites">
        <rdfs:label xml:lang="en">cites</rdfs:label>
        <skos:definition xml:lang="en">Visual citation : an artistic process/practice where a
            creator reproduces the totality or a section of a (well-known) work of art to
            incorporate it a new visual creation.</skos:definition>
        <rdfs:subPropertyOf rdf:resource="http://id.loc.gov/ontologies/bibframe/relatedTo"/>
        <owl:inverseOf rdf:resource="http://artframe.biblioteko-o.org/citedBy"/>
    </owl:ObjectProperty>

    <owl:ObjectProperty rdf:about="http://artframe.biblioteko-o.org/citedBy">
        <rdfs:label xml:lang="en">is cited by</rdfs:label>
        <skos:definition xml:lang="en">Visual citation : an artistic process/practice where a
            creator reproduces the totality or a section of a (well-known) work of art to
            incorporate it a new visual creation.</skos:definition>
        <rdfs:subPropertyOf rdf:resource="http://id.loc.gov/ontologies/bibframe/relatedTo"/>
        <owl:inverseOf rdf:resource="http://artframe.biblioteko-o.org/cites"/>
    </owl:ObjectProperty>

    <owl:ObjectProperty rdf:about="http://artframe.biblioteko-o.org/onCarrierWith">
        <rdfs:label xml:lang="en">on carrier with</rdfs:label>
        <skos:definition xml:lang="en">A resource is contained on the same carrier as the resource
            being described</skos:definition>
        <rdfs:subPropertyOf rdf:resource="http://id.loc.gov/ontologies/bibframe/relatedTo"/>
    </owl:ObjectProperty>

    <owl:ObjectProperty rdf:about="http://artframe.biblioteko-o.org/describes">
        <rdfs:label xml:lang="en">describes</rdfs:label>
        <skos:definition xml:lang="en">This resource provides a description of another, for example
            a ConditionAssessment describes a PhysicalCondition.</skos:definition>
        <owl:inverseOf rdf:resource="http://artframe.biblioteko-o.org/describedBy"/>
    </owl:ObjectProperty>

    <owl:ObjectProperty rdf:about="http://artframe.biblioteko-o.org/describedBy">
        <rdfs:label xml:lang="en">described by</rdfs:label>
        <skos:definition xml:lang="en">This resource is described by another, for example a
            PhysicalCondition is described by a ConditionAssessment</skos:definition>
        <owl:inverseOf rdf:resource="http://artframe.biblioteko-o.org/describes"/>
    </owl:ObjectProperty>

    <owl:ObjectProperty rdf:about="http://artframe.biblioteko-o.org/hasInput">
        <rdfs:label xml:lang="en">has input</rdfs:label>
        <skos:definition xml:lang="en">One resource has another resource as input, for example when
            one resource is informed or acted on by another. A ConservatorActivity has input from a
            ConditionAssessment.</skos:definition>
        <owl:inverseOf rdf:resource="http://artframe.biblioteko-o.org/isInputTo"/>
    </owl:ObjectProperty>

    <owl:ObjectProperty rdf:about="http://artframe.biblioteko-o.org/isInputTo">
        <rdfs:label xml:lang="en">is input to</rdfs:label>
        <skos:definition xml:lang="en">One resource provides input to another. For example, a
            ConditionAssessment provides input to a ConservatorActivity.</skos:definition>
        <owl:inverseOf rdf:resource="http://artframe.biblioteko-o.org/hasInput"/>
    </owl:ObjectProperty>
    
    <owl:ObjectProperty rdf:about="http://artframe.biblioteko-o.org/hasPhysicalCondition">
        <rdfs:label xml:lang="en">has physical condition</rdfs:label>
        <skos:definition xml:lang="en">Relates an object or part of an object to a specific aspect of its physical condition.</skos:definition>
        <rdfs:range rdf:resource="http://artframe.biblioteko-o.org/PhysicalCondition"/>
        <owl:inverseOf rdf:resource="http://artframe.biblioteko-o.org/isPhysicalConditionOf"/>
    </owl:ObjectProperty>
    
    <owl:ObjectProperty rdf:about="http://artframe.biblioteko-o.org/isPhysicalConditionOf">
        <rdfs:label xml:lang="en">is physical condition of</rdfs:label>
        <skos:definition xml:lang="en">Relates a specific physical condition to an object or part of an object.</skos:definition>
        <rdfs:domain rdf:resource="http://artframe.biblioteko-o.org/PhysicalCondition"/>
        <owl:inverseOf rdf:resource="http://artframe.biblioteko-o.org/hasPhysicalCondition"/>
    </owl:ObjectProperty>

    <!-- NAMED INDIVIDUALS -->

</rdf:RDF>
